---
title: "Sufficient Statistic"
engine: knitr
format: 
  html: default
  pdf: default
---



## Sufficient Statistics

::: {#def-sufficient-statistic}

### Sufficient Statistic
A statistic $T=T(X)$ is sufficient for $\theta$ if one of the following three equivalent conditions holds:

1.  **Paralell Log-Likelihood:**
   
    For any pair of data sets $x$ and $y$ such that $T(x)=T(y)$, the difference in their log-likelihoods ($\ell(\theta;x)=\ln(f(x;\theta)))$ is constant with respect to $\theta$:
    $$
    \ell(\theta; x) - \ell(\theta; y) = c(x, y) \quad \text{for all } \theta
    $$
    where $c(x,y)$ depends only on $x$ and $y$, not on $\theta$.

2.  **Factorization of likelihood:**
   The likelihood function of $\theta$ given $x$ can be expressed as:
    $$
    L(\theta; x) = h(x)g(t(x);\theta)
    $$
    where $h(x)$ is irrelevant to $\theta$. 


3.  **Non-informative Conditional Distribution of $X|T(X)$:**
   
    The conditional distribution of $X$ given $T(X)=t$, denoted as $f(x|t(x), \theta)$, is independent of $\theta$.
    $$
    f(x|t(x), \theta) = f(x|t(x))
    $$

:::


```{r }
#| label: fig-par-log-likelihood
#| fig-cap: "Visualizing Parallel Log-Likelihoods"
#| echo: false
#| fig-align: "center"
#| message: false
#| warning: false
#| out.width: "70%"

library(ggplot2)

# Define range for theta
theta <- seq(0, 6, length.out = 300)

# Define log-likelihood functions

# Peak is set exactly at y = 4 to align with a grid line
ll_x <- -0.8 * (theta - 3)^2 + 4 

# The gap is set to 2, matching the grid spacing
const_diff <- 2
ll_y <- ll_x - const_diff

# Create data frame for plotting

# We use simple factor levels "A" and "B" for mapping, 

# then swap them for expressions in the scale functions
df <- data.frame(
  theta = rep(theta, 2),
  loglik = c(ll_x, ll_y),
  curve = rep(c("A", "B"), each = 300)
)

# Plot
ggplot(df, aes(x = theta, y = loglik, color = curve, linetype = curve)) +
  geom_line(linewidth = 1.2) +
  
  # Styling with Math Expressions in Legends
  scale_color_manual(
    values = c("blue", "red"),
    labels = expression(l(theta*"; "*x), l(theta*"; "*y))
  ) +
  scale_linetype_manual(
    values = c("solid", "dashed"),
    labels = expression(l(theta*"; "*x), l(theta*"; "*y))
  ) +
  
  # Force grid lines to align with the peaks and the gap
  scale_y_continuous(breaks = seq(-10, 10, by = 2)) +
  
  # Math expressions for axes
  labs(x = expression(theta), 
       y = expression(l(theta)),
       title = "Parallel Log-Likelihoods",
       subtitle = "Vertical difference is constant everywhere") +
  
  theme_minimal() +
  theme(legend.title = element_blank(),
        legend.position = "top",
        text = element_text(size = 12),
        plot.title = element_text(size = 12, face = "bold"),
        panel.grid.major.y = element_line(color = "gray60", linetype = "dotted"),
        panel.grid.minor.y = element_blank())

```

:::{#thm-paralell-loglik}
### Factorization Theorem
The three conditions in the definitions of @def-sufficient-statistic are equivalent. 
:::

<details>
<summary>Click to view Complete Proof of Equivalence</summary>

::: {.proof}
**Proof of Equivalence**

We show the equivalence by proving the implications in a cycle or pairs: $(2 \Rightarrow 1)$, $(1 \Rightarrow 2)$, $(2 \Rightarrow 3)$, and $(3 \Rightarrow 2)$.

1. Factorization $\Rightarrow$ Log-Likelihood Difference $(2 \Rightarrow 1)$

Assume the **Factorization Theorem** holds: $L(\theta; x) = h(x) g(T(x); \theta)$.
Consider any pair $x, y$ such that $T(x) = T(y)$.
$$
\ell(\theta; x) - \ell(\theta; y) = [\ln h(x) + \ln g(T(x); \theta)] - [\ln h(y) + \ln g(T(y); \theta)]
$$
Since $T(x)=T(y)$, the terms $\ln g(T(x); \theta)$ and $\ln g(T(y); \theta)$ are identical and cancel out.
$$
\ell(\theta; x) - \ell(\theta; y) = \ln h(x) - \ln h(y)
$$
This difference depends only on $x$ and $y$ (via $h$), and is independent of $\theta$. Thus, condition 1 holds.

2. Log-Likelihood Difference $\Rightarrow$ Factorization $(1 \Rightarrow 2)$

Assume Condition 1 holds. For any $x$ and $y$ with $T(x)=T(y)$, $\ell(\theta; x) - \ell(\theta; y) = c(x, y)$.
Exponentiating, we get $L(\theta; x) = k(x, y) L(\theta; y)$, where $k$ is independent of $\theta$.

For each value $t$ in the range of $T$, select a fixed representative data point $x_t$ such that $T(x_t) = t$.
For any data point $x$, let $t = T(x)$. Using the relation above:
$$
L(\theta; x) = k(x, x_t) L(\theta; x_t)
$$
Define $h(x) = k(x, x_{T(x)})$ and $g(t; \theta) = L(\theta; x_t)$.
Then:
$$
L(\theta; x) = h(x) g(T(x); \theta)
$$
This is exactly the Factorization form.

3. Factorization $\Rightarrow$ Conditional Distribution $(2 \Rightarrow 3)$

Assume $f(x; \theta) = h(x)g(T(x); \theta)$. We derive the conditional distribution $P(X=x | T(X)=t)$.
If $T(x) \neq t$, the probability is 0 (independent of $\theta$).
If $T(x) = t$:
$$
P(X=x | T(X)=t) = \frac{P(X=x, T(X)=t)}{P(T(X)=t)} = \frac{f(x; \theta)}{\sum_{\{y : T(y)=t\}} f(y; \theta)}
$$
Substitute the factorization:
$$
= \frac{h(x)g(t; \theta)}{\sum_{\{y : T(y)=t\}} h(y)g(t; \theta)} = \frac{h(x)g(t; \theta)}{g(t; \theta) \sum_{\{y : T(y)=t\}} h(y)}
$$
The term $g(t; \theta)$ cancels out:
$$
= \frac{h(x)}{\sum_{\{y : T(y)=t\}} h(y)}
$$
This expression depends only on $x$ and $h(\cdot)$, and is entirely free of $\theta$. Thus, Condition 3 holds.

4. Conditional Distribution $\Rightarrow$ Factorization $(3 \Rightarrow 2)$

Assume $f(x | T(x); \theta) = k(x)$, where $k(x)$ is independent of $\theta$.
We can write the joint distribution as:
$$
f(x; \theta) = f(x | T(x)=t; \theta) \cdot P(T(X)=t; \theta)
$$
Substitute the assumption:
$$
f(x; \theta) = k(x) \cdot P(T(X)=T(x); \theta)
$$
Let $h(x) = k(x)$ and $g(t; \theta) = P(T(X)=t; \theta)$.
Then:
$$
f(x; \theta) = h(x) g(T(x); \theta)
$$
This recovers the Factorization form.

:::

</details>

::: {#exm-uniform-sufficiency}

### Uniform Distribution $U(\theta-1, \theta+1)$
Consider a random sample $X_1, \dots, X_n$ from a Uniform distribution with range $(\theta-1, \theta+1)$.

The density for a single observation is:

$$
f(x_i|\theta) = \frac{1}{(\theta+1) - (\theta-1)} I(\theta-1 < x_i < \theta+1) = \frac{1}{2} I(\theta-1 < x_i < \theta+1)
$$

The joint PDF (likelihood) is:

$$
L(\theta; x) = \prod_{i=1}^n \frac{1}{2} I(\theta-1 < x_i < \theta+1)
$$

$$
L(\theta; x) = 2^{-n} \cdot I( \min(x_i) > \theta-1 ) \cdot I( \max(x_i) < \theta+1 )
$$

Using order statistics notation where $X_{(1)} = \min(X_i)$ and $X_{(n)} = \max(X_i)$:

$$
L(\theta; x) = 2^{-n} \cdot I( \theta < X_{(1)} + 1 ) \cdot I( \theta > X_{(n)} - 1 )
$$

$$
L(\theta; x) = 2^{-n} \cdot I( X_{(n)} - 1 < \theta < X_{(1)} + 1 )
$$

By the **Factorization Theorem**, we can define:

* $h(x) = 2^{-n}$ (or simply 1, grouping constants into $g$)
   * $g(T(x), \theta) = I( X_{(n)} - 1 < \theta < X_{(1)} + 1 )$

Thus, the sufficient statistic is the pair of order statistics:
$$
T(X) = (X_{(1)}, X_{(n)})
$$

:::


::: {#exm-gamma-sufficiency}

### Gamma Distribution
Let $X_1, \dots, X_n$ be i.i.d. $\Gamma(\alpha, \beta)$. The pdf is:

$$
f(x|\alpha, \beta) = \frac{1}{\Gamma(\alpha)\beta^\alpha} x^{\alpha-1} e^{-x/\beta}, \quad x > 0
$$

The joint likelihood is:

$$
L(\alpha, \beta; x) = \left( \frac{1}{\Gamma(\alpha)\beta^\alpha} \right)^n \left( \prod_{i=1}^n x_i \right)^{\alpha-1} \exp\left( -\frac{1}{\beta} \sum_{i=1}^n x_i \right)
$$

By the Factorization Theorem, we can identify the parts that depend on the data and the parameters:
$$
g(T(x), \theta) = \left( \prod_{i=1}^n x_i \right)^{\alpha} \exp\left( -\frac{1}{\beta} \sum_{i=1}^n x_i \right)
$$

Thus, the sufficient statistics are:
$$
T(X) = \left( \prod_{i=1}^n X_i, \sum_{i=1}^n X_i \right)
$$

:::


::: {#exm-exp-family-sufficiency}

### General Exponential Family
Many common distributions (Normal, Poisson, Gamma, Binomial) belong to the Exponential Family. The lecture notes (Page 7) note that if a density can be written in the form:

$$
f(x|\theta) = h(x) c(\theta) \exp\left( \sum_{j=1}^k w_j(\theta) t_j(x) \right)
$$

Then, by the Factorization Theorem, the statistic:

$$
T(X) = \left( \sum_{i=1}^n t_1(x_i), \dots, \sum_{i=1}^n t_k(x_i) \right)
$$

is a sufficient statistic for $\theta$.


:::

::: {#exm-bernoulli-expfamily}

### Bernoulli as Exponential Family
Let $X_1, \dots, X_n \overset{i.i.d.}{\sim} \text{Bernoulli}(p)$.
To find the sufficient statistic, we write the joint density in the canonical **Exponential Family** form:
$$
f(x; \theta) = h(x) \exp\left( \eta(\theta) T(x) - A(\theta) \right)
$$

1. Write the Joint PDF:
    $$
f(x|p) = \prod_{i=1}^n p^{x_i} (1-p)^{1-x_i}
$$

2. Convert to Exponential Form:
    $$
\begin{aligned}
f(x|p) &= \exp\left( \ln \left( \prod_{i=1}^n p^{x_i} (1-p)^{1-x_i} \right) \right) \\
&= \exp\left( \sum_{i=1}^n \left[ x_i \ln p + (1-x_i) \ln(1-p) \right] \right) \\
&= \exp\left( (\ln p) \sum x_i + \ln(1-p) \left( n - \sum x_i \right) \right)
\end{aligned}
$$

3. Group Terms by $x$ and $p$:
    $$
\begin{aligned}
f(x|p) &= \exp\left( \underbrace{\left( \ln p - \ln(1-p) \right)}_{\eta(p)} \underbrace{\left(\sum_{i=1}^n x_i\right)}_{T(x)} + \underbrace{n \ln(1-p)}_{-A(p)} \right)
\end{aligned}
$$

**Conclusion:**
By the structure of the exponential family, the term multiplying the natural parameter $\eta(p) = \ln\left(\frac{p}{1-p}\right)$ is the sufficient statistic:
$$
T(X) = \sum_{i=1}^n X_i
$$

:::


::: {#rem-sufficient-likelihood}

### Sufficient Statistic as Parameter of Likelihood
There is a dual relationship between the sufficient statistic and the parameter $\theta$. Conventionally, we view $f(x|\theta)$ as a function of $x$ parameterized by $\theta$.

However, in Bayesian inference or likelihood theory, we often view the likelihood $L(\theta; x)$ as a function of $\theta$ determined by the observed data $x$. The Factorization Theorem implies:

$$
L(\theta; \mathbf{x}) \propto g(T(\mathbf{x})|\theta)
$$

This suggests that $T(\mathbf{x})$ completely determines the shape of the likelihood function. In this specific sense, the sufficient statistic $T(\mathbf{x})$ acts as the **"parameter"** of the likelihood function itself.

For the exponential family that we will discuss below, this duality is explicit:

$$
\log L(\theta; \mathbf{x}) = \text{const} + \sum_{i=1}^k \eta_i(\theta) T_i(\mathbf{x}) - n A(\theta)
$$

Here, $T_i(\mathbf{x})$ serves as the coefficient (or parameter) for the function $\eta_i(\theta)$.

:::

## Minimal Sufficient Statistic

::: {#def-mss}

### Minimal Sufficient Statistic (MSS)
A statistic $T(X)$ is a **Minimal Sufficient Statistic** if:

1.  **Sufficiency:** $T(X)$ is a sufficient statistic for $\theta$.
   2.  **Minimality:** For any other sufficient statistic $S(X)$, $T(X)$ is a function of $S(X)$.
    $$
    T(X) = g(S(X))
    $$
    *(This implies that $T(X)$ provides the greatest possible data reduction without losing information about $\theta$. If $S(x) = S(y)$, then it must be that $T(x) = T(y)$).*

:::

::: {#thm-mss-loglik}

### MSS Condition Theorem
Let $T(X)$ be a **sufficient statistic**. $T(X)$ is a **Minimal Sufficient Statistic (MSS)** if and only if for any pair of data sets $x$ and $y$:
$$
\ell(\theta; x) = \ell(\theta; y) + c(x, y) \text{ for all } \theta \implies T(x) = T(y)
$$
where $c(x, y)$ is a constant independent of $\theta$.

:::

<details>
<summary>Click to view the Proof</summary>

::: {.proof}


**Direction 1: Sufficiency (Implication holds $\implies$ $T$ is MSS)**

Assume that for any $x, y$, $[\ell(\theta; x) = \ell(\theta; y) + c(x, y)] \implies T(x) = T(y)$. We must show that $T$ is a function of *any* sufficient statistic $U$.

1.  Let $U(X)$ be any sufficient statistic. Assume $U(x) = U(y)$.
   2.  By the **Factorization Theorem**, the likelihoods are:
    $$
    L(\theta; x) = h(x)g(U(x), \theta)
    $$
    $$
    L(\theta; y) = h(y)g(U(y), \theta)
    $$

3.  Since $U(x) = U(y)$, the factor $g(U(x), \theta)$ is identical to $g(U(y), \theta)$.
    Taking the log-ratio:
    $$
    \ell(\theta; x) - \ell(\theta; y) = \ln h(x) - \ln h(y)
    $$
    The term $\ln h(x) - \ln h(y)$ depends only on $x$ and $y$, not on $\theta$. Let this be $c(x,y)$.
    $$
    \ell(\theta; x) = \ell(\theta; y) + c(x, y)
    $$

4.  By our main assumption, this condition implies $T(x) = T(y)$.
   5.  Thus, we have shown that $U(x) = U(y) \implies T(x) = T(y)$. This means $T$ is a function of $U$.
    Since $U$ is arbitrary, $T$ is Minimal Sufficient.

**Direction 2: Necessity ($T$ is MSS $\implies$ Implication holds)**

Assume $T$ is Minimal Sufficient. We must prove that if $\ell(\theta; x) = \ell(\theta; y) + c(x, y)$ for all $\theta$, then $T(x) = T(y)$.

1.  **Define the Statistic $S(x)$:**
    Let $S(x)$ be the set of all possible datasets $z$ which give the same log-likelihood shape as $x$:
    $$
    S(x) = \{z \mid \ell(\theta; z) = \ell(\theta; x) + c_z \text{ for all } \theta \}
    $$
    This statistic $S(x)$ represents the equivalence class of $x$ under the parallel log-likelihood relationship.
    If the condition $\ell(\theta; x) = \ell(\theta; y) + c(x, y)$ holds, then by definition $x$ and $y$ generate the same equivalence class, so $S(x) = S(y)$.

2.  **Show $S(x)$ is Sufficient (Directly via Likelihood Ratio):**
    To prove $S$ is sufficient, we check the **Likelihood Ratio Condition** (Condition 2 from Section 1.1).
    Suppose $S(x) = S(y)$. By the definition of $S$, this implies:
    $$
    \ell(\theta; x) - \ell(\theta; y) = c(x, y)
    $$
    By the definition of sufficiency, $S(X)$ is a sufficient statistic.

3.  **Use Minimality of $T$:**
    Since $T$ is a **Minimal** Sufficient Statistic, it is a function of *any* sufficient statistic.
    Therefore, $T$ must be a function of $S$. That is, $T(x) = f(S(x))$.

4.  **Conclusion:**
    Assume $\ell(\theta; x) = \ell(\theta; y) + c(x, y)$.
    Then $S(x) = S(y)$.
    Consequently, $T(x) = f(S(x)) = f(S(y)) = T(y)$.

:::

</details>


::: {#exm-bernoulli-mss-check}

### Checking Minimality via Log-Likelihood Condition
Let $X_1, X_2, X_3 \overset{i.i.d.}{\sim} \text{Bernoulli}(p)$.
We determine the MSS by checking the implication from the **MSS Condition Theorem**:
$$
\text{Parallel Log-Likelihoods} \implies T(x) = T(y)
$$

**Step 1: Establishing the MSS**
First, we find the condition under which two log-likelihoods are parallel.
$$
\ell(p; x) = (\sum x_i) \ln p + (n - \sum x_i) \ln(1-p)
$$
The difference $\ell(p; x) - \ell(p; y)$ depends on $p$ only through the term $(\sum x_i - \sum y_i) \ln \frac{p}{1-p}$.
For this difference to be constant (independent of $p$), the coefficient must be zero:
$$
\text{Parallel Log-Likelihoods} \iff \sum x_i = \sum y_i
$$
The statistic that corresponds exactly to this condition is $T(X) = \sum X_i$.
Since $\sum x_i = \sum y_i$ trivially implies $T(x) = T(y)$, $T(X)$ is the **Minimal Sufficient Statistic**.

**Step 2: Why $S(X) = (X_1, \sum_{i=2}^3 X_i)$ is NOT Minimal**
Now consider the "richer" statistic $S(X)$. If $S$ were minimal, the parallel condition must imply $S(x) = S(y)$.
We check:
$$
\sum x_i = \sum y_i \stackrel{?}{\implies} (x_1, \sum_{i=2}^3 x_i) = (y_1, \sum_{i=2}^3 y_i)
$$
**Counter-Example:**
Let $x = (1, 0, 1)$ and $y = (0, 1, 1)$.

1.  **Check Parallel Condition:**
    $\sum x_i = 2$ and $\sum y_i = 2$.
    The sums are equal, so the log-likelihoods are parallel.

2.  **Check Statistic Equality:**
    $$S(x) = (1, 1)$$
    $$S(y) = (0, 2)$$
    $$S(x) \neq S(y)$$

**Conclusion:** The parallel condition holds, but $S(x) \neq S(y)$. The implication fails.
This proves that $S(X)$ is **not** minimalâ€”it retains "extra" information (the position of the first success) that is not relevant to the likelihood shape.

:::